src/computational_monads/simulation_semantics/constructions/query_log.lean
@@ -1,0 +1,277 @@
+import computational_monads.oracle_spec
+
+/-- Data type representing a log of oracle queries for a given `oracle_spec`.
+  Represented as a list of query inputs and outputs, indexed by the indexing set in the spec -/
+def query_log (spec : oracle_spec) : Type :=
+  Π (i : spec.ι), list (spec.domain i × spec.range i)
+
+namespace query_log
+
+variables {spec : oracle_spec} (log : query_log spec)
+
+section init
+
+/-- Empty query log, with no entries for any of the oracles in the spec -/
+@[inline, reducible]
+def init (spec : oracle_spec) : query_log spec :=
+λ i, []
+
+@[simp]
+lemma init_apply (spec : oracle_spec) (i : spec.ι) :
+  (init spec) i = [] :=
+rfl
+
+end init
+
+section log_query
+
+variable [spec.computable] 
+
+/-- Given a current query log, return the new log after adding a given oracle query -/
+def log_query (log : query_log spec) (i : spec.ι) (t : spec.domain i) (u : spec.range i) :
+  query_log spec :=
+λ j, if hi : i = j then hi.rec_on ((t, u) :: (log i)) else log j
+
+lemma log_query_apply (i j : spec.ι) (t : spec.domain i) (u : spec.range i) :
+  (log.log_query i t u) j = if hi : i = j then hi.rec_on ((t, u) :: log i) else log j :=
+rfl
+
+lemma log_query_apply_of_index_eq (log : query_log spec)
+  {i j : spec.ι} (hi : i = j) (t : spec.domain i) (u : spec.range i) :
+  (log.log_query i t u) j = hi.rec_on ((t, u) :: log i) :=
+dite_eq_iff.2 (or.inl ⟨hi, rfl⟩)
+
+@[simp]
+lemma log_query_apply_same_index (log : query_log spec)
+  (i : spec.ι) (t : spec.domain i) (u : spec.range i) :
+  (log.log_query i t u) i = (t, u) :: (log i) :=
+log_query_apply_of_index_eq log rfl t u
+
+lemma log_query_apply_of_index_ne (log : query_log spec)
+  {i j : spec.ι} (hi : i ≠ j) (t : spec.domain i) (u : spec.range i) :
+  (log.log_query i t u) j = log j :=
+dite_eq_iff.2 (or.inr ⟨hi, rfl⟩)
+
+end log_query
+
+section lookup
+
+variable [spec.computable]
+
+/-- Find the query output of the first oracle query with the given input.
+  Result is returned as an `option`, with `none` for inputs that haven't previously been queried -/
+def lookup (log : query_log spec) (i : spec.ι) (t : spec.domain i) :
+  option (spec.range i) :=
+((log i).find $ (= t) ∘ prod.fst).map prod.snd
+
+@[simp]
+lemma lookup_init (spec : oracle_spec) [spec.computable]
+  (i : spec.ι) (t : spec.domain i) :
+  (init spec).lookup i t = none :=
+option.map_none'
+
+/-- Most general version of the lemma is somewhat cumbersome because of the equality induction.
+  More specific versions given below are usually more usefull -/
+lemma lookup_log_query (i j : spec.ι)
+  (t : spec.domain i) (t' : spec.domain j) (u : spec.range i) :
+  (log.log_query i t u).lookup j t' = if hi : i = j
+    then (if hi.rec_on t = t' then hi.rec_on (some u) else log.lookup j t')
+    else log.lookup j t' := 
+begin
+  split_ifs with hi ht,
+  { induction hi, induction ht,
+    simp only [lookup, log_query_apply_same_index,
+      list.find_cons_of_pos, function.comp_app, option.map_some'] },
+  { induction hi,
+    refine congr_arg (option.map prod.snd) _,
+    refine (log.log_query_apply_same_index i t u).symm ▸ _,
+    exact list.find_cons_of_neg (log i) ht },
+  { refine congr_arg (option.map prod.snd ∘ _) _,
+    exact (log.log_query_apply_of_index_ne hi t u) }
+end
+
+@[simp]
+lemma lookup_log_query_same_index (i : spec.ι)
+  (t t' : spec.domain i) (u : spec.range i) :
+  (log.log_query i t u).lookup i t' = if t = t' then some u else log.lookup i t' :=
+trans (log.lookup_log_query  i i t t' u) (dif_pos rfl)
+
+lemma lookup_log_query_of_index_ne (i j : spec.ι) (hi : i ≠ j)
+  (t : spec.domain i) (t' : spec.domain j) (u : spec.range i) :
+  (log.log_query i t u).lookup j t' = log.lookup j t' :=
+trans (log.lookup_log_query i j t t' u) (dif_neg hi)
+
+@[simp]
+lemma lookup_log_query_same_input (i : spec.ι)
+  (t : spec.domain i) (u : spec.range i) :
+  (log.log_query i t u).lookup i t = some u :=
+trans (log.lookup_log_query_same_index i t t u) (if_pos rfl)
+
+lemma lookup_log_query_of_input_ne (i : spec.ι)
+  (t t' : spec.domain i) (ht : t ≠ t') (u : spec.range i) :
+  (log.log_query i t u).lookup i t' = log.lookup i t' :=
+trans (log.lookup_log_query_same_index i t t' u) (if_neg ht)
+
+end lookup
+
+section remove_head
+
+variable [spec.computable]
+
+-- remove the head of the index `i` log
+def remove_head (log : query_log spec) (i : spec.ι) :
+  query_log spec :=
+λ j, if i = j then (log j).tail else (log j)
+
+@[simp]
+lemma remove_head_apply (i j : spec.ι) :
+  log.remove_head i j = if i = j then (log j).tail else (log j) :=
+rfl
+
+lemma remove_head_apply_of_index_eq {i j : spec.ι} (hi : i = j) :
+  log.remove_head i j = (log j).tail :=
+if_pos hi
+
+@[simp]
+lemma remove_head_apply_same_index (i : spec.ι) :
+  log.remove_head i i = (log i).tail :=
+log.remove_head_apply_of_index_eq rfl
+
+lemma remove_head_apply_of_index_ne {i j : spec.ι} (hi : i ≠ j) :
+  log.remove_head i j = log j :=
+if_neg hi
+
+@[simp]
+lemma remove_head_init (spec : oracle_spec) [spec.computable] (i : spec.ι) :
+  (init spec).remove_head i = init spec :=
+funext (λ i', if_t_t (i = i') [])
+
+lemma remove_head_log_query (i j : spec.ι)
+  (t : spec.domain i) (u : spec.range i) :
+  (log.log_query i t u).remove_head j =
+    if hi : i = j then log else (log.remove_head j).log_query i t u :=
+begin
+  split_ifs with hi,
+  { induction hi,
+    refine (funext $ λ k, trans (remove_head_apply _ i k) _),
+    split_ifs with hk,
+    { induction hk,
+      rw [log_query_apply_same_index log, list.tail_cons] },
+    { exact log_query_apply_of_index_ne log hk t u } },
+  { refine (funext $ λ k, _),
+    simp only [remove_head_apply],
+    split_ifs with hj,
+    { induction hj,
+      simp only [log_query_apply_of_index_ne _ hi, remove_head_apply_same_index] },
+    { simp only [log_query_apply, remove_head_apply_of_index_ne _ hj,
+        remove_head_apply_of_index_ne _ (ne.symm hi)] } }
+end
+
+lemma remove_head_log_query_apply_of_index_eq {i j : spec.ι} (hi : i = j)
+  (t : spec.domain i) (u : spec.range i) :
+  (log.log_query i t u).remove_head j = log :=
+trans (log.remove_head_log_query i j t u) (if_pos hi)
+
+@[simp]
+lemma remove_head_log_query_apply_of_same_index (i : spec.ι)
+  (t : spec.domain i) (u : spec.range i) :
+  (log.log_query i t u).remove_head i = log :=
+log.remove_head_log_query_apply_of_index_eq rfl t u
+
+lemma remove_head_log_query_apply_of_index_ne {i j : spec.ι} (hi : i ≠ j)
+  (t : spec.domain i) (u : spec.range i) :
+  (log.log_query i t u).remove_head j = (log.remove_head j).log_query i t u :=
+trans (log.remove_head_log_query i j t u) (if_neg hi)
+
+end remove_head
+
+section not_queried
+
+variable [spec.computable]
+
+-- Check that a input was never queried
+def not_queried (log : query_log spec) (i : spec.ι) (t : spec.domain i) : bool :=
+((log i).find ((=) t ∘ prod.fst)).is_none
+
+lemma not_queried_def (i : spec.ι) (t : spec.domain i) :
+  log.not_queried i t = ((log i).find ((=) t ∘ prod.fst)).is_none :=
+rfl
+
+lemma not_queried_init_eq_tt (spec : oracle_spec) [spec.computable]
+  (i : spec.ι) (t : spec.domain i) :
+  (init spec).not_queried i t = tt :=
+rfl
+
+lemma not_queried_log_query (i j : spec.ι)
+  (t : spec.domain i) (t' : spec.domain j) (u : spec.range i) :
+  (log.log_query i t u).not_queried j t' =
+    (log.not_queried j t') && (if hi : i = j then (hi.rec_on t ≠ t') else tt) :=
+begin
+  split_ifs with hi,
+  { induction hi,
+    rw [not_queried, log_query_apply_same_index],
+    by_cases ht : t' = t,
+    { induction ht,
+      have : (eq t' ∘ prod.fst) (t', u) := (function.comp_app (eq t') prod.fst (t', u)).symm ▸ rfl,
+      simp only [list.find_cons_of_pos _ this, option.is_none_some, ne.def, eq_self_iff_true,
+        not_true, to_bool_false_eq_ff, band_ff] },
+    { have : ¬ (eq t' ∘ prod.fst) (t, u) := by simp only [ht, function.comp_app, not_false_iff],
+      simpa only [list.find_cons_of_neg _ this, ht, ne.symm ht,
+        ne.def, not_false_iff, to_bool_true_eq_tt, band_tt] } },
+  { simp only [not_queried, log_query_apply_of_index_ne log hi, band_tt] }
+end
+
+lemma not_queried_log_query_of_index_eq {i j : spec.ι} (hi : i = j)
+  (t : spec.domain i) (t' : spec.domain j) (u : spec.range i) :
+  (log.log_query i t u).not_queried j t' = (log.not_queried j t') && (hi.rec_on t ≠ t') :=
+(log.not_queried_log_query i j t t' u).trans (congr_arg ((&&) $ log.not_queried j t') (dif_pos hi))
+
+lemma not_queried_log_query_same_index (i : spec.ι)
+  (t t' : spec.domain i) (u : spec.range i) :
+  (log.log_query i t u).not_queried i t' = (log.not_queried i t') && (t ≠ t') :=
+log.not_queried_log_query_of_index_eq rfl t t' u
+
+lemma not_queried_log_query_of_index_ne {i j : spec.ι} (hi : i ≠ j)
+  (t : spec.domain i) (t' : spec.domain j) (u : spec.range i) :
+  (log.log_query i t u).not_queried j t' = log.not_queried j t' :=
+(log.not_queried_log_query i j t t' u).trans 
+  ((congr_arg _ (dif_neg hi)).trans (band_tt _))
+
+end not_queried
+
+section to_seed
+
+/-- Wrapping function that just reverses every list in the given `query_log`. 
+  Intended to turn a log into something that can be used as a seed for a computation.
+  Needed because the logging function adds the new queries to the front  -/
+def to_seed (log : query_log spec) :
+  query_log spec :=
+λ i, (log i).reverse
+
+end to_seed
+
+-- Different lookup that only looks at head, and removes the element from the cache
+def take_fst [spec.computable]
+  (log : query_log spec) (i : spec.ι) (t : spec.domain i) :
+  option (spec.range i) × query_log spec :=
+match (log i).nth 0 with
+| none := (none, query_log.init spec)
+| some ⟨t', u⟩ := if t' = t then (some u, log.remove_head i)
+    else (none, query_log.init spec) -- TODO: maybe don't clear everything here?
+end
+
+/-- Get the index of the given input, with depth at most equal to the given number `q`.
+  In most applications `q` will be the maximum number of queries that a computation makes.
+  This allows the result to be bounded and therefore returned as a `fin q` rather than a `ℕ` -/
+def get_index [spec.computable] (log : query_log spec)
+  (i : spec.ι) (t : spec.domain i) (q : ℕ) : option (fin q) :=
+match (log i) with
+| [] := none
+| ((t', u) :: ls) := sorry
+end 
+
+/-- Remove parts of the cache after the query chosen to fork on -/
+def fork_cache {q : ℕ} {T U : Type} [inhabited U] : (option $ fin q) → query_log (T →ₒ U) → query_log (T →ₒ U)
+:= sorry -- TODO: This is essentially in the `query_log.lean` file but needs a few modifications
+
+end query_log
